finish completeness of wf_kind

SystemFD/Algorithm/Completeness1.lean
@@ -3,60 +3,88 @@ import SystemFD.Judgment
 import SystemFD.Ctx
 import SystemFD.Algorithm
 import SystemFD.Metatheory.Classification
+import SystemFD.Metatheory.Shape
 
 set_option maxHeartbeats 500000
 
 @[simp]
-abbrev WfKindCompleteType : (v : JudgmentVariant) -> Ctx Term -> JudgmentArgs v -> Prop
-| .prf => λ Γ => λ (t, τ) => τ = .kind -> Γ = [] -> Γ ⊢ t : τ -> wf_kind t = .some ()
+abbrev WfKindCompleteLemmaType : (v : JudgmentVariant) -> Ctx Term -> JudgmentArgs v -> Prop
+| .prf => λ Γ => λ (t, A) => A = □ -> Γ ⊢ t : A -> wf_kind t = .some ()
 | .wf  => λ _ => λ () => true
 
-
-theorem wf_kind_complete :
-  ⊢ Γ ->
+theorem wf_kind_complete_lemma :
   Judgment v Γ idx ->
-  WfKindCompleteType v Γ idx
+  WfKindCompleteLemmaType v Γ idx
 := by
-intros wf j; induction j <;> simp at *;
-case _ =>
-  intro e1 e2 h; subst e1; subst e2
-  cases h; case _ h _ => cases h
-case _ gt _ =>
-  intro e1 e2 h; subst e1; subst e2;
-  case _ =>
-  cases gt;
-case _ h1 h2 ih1 ih2 =>
-  intro e2 h; subst e2;
-  rw[Option.bind_eq_some]; exists ();
-  replace ih1 := ih1 wf rfl h1
-  replace ih2 := ih2 wf rfl h2
-  apply And.intro;
-  assumption
-  rw[Option.bind_eq_some]; exists ();
-case _ =>
-  intro e; subst e;
-  case _ j =>
-  have lem := classification_lemma j; simp at lem;
-  cases lem;
-  case _ h => cases h; case _ h => cases h
-  case _ h =>
-    cases h; case _ w h =>
-    cases h; case _ w1 h =>
-    cases h; cases w1
-case _ =>
-  intro e1 e2; subst e1; subst e2
-  intro h;
-  cases h; case _ h _ => cases h;
-case _ =>
-  intro e h; subst e;
-  cases h; case _ h => cases h;
-all_goals (
-  intro e1 e2 h; subst e1; subst e2;
-  cases h;
-)
-case _ h =>
-  sorry
-case _ h =>
-  sorry
-case _ h =>
-  sorry
+intro j; induction j <;> simp at *
+case letterm j1 j2 j3 j4 ih1 ih2 ih3 ih4 =>
+  intro h1 h2; subst h1
+  cases j4
+case var Γ x _ j1 j2 _  =>
+  intro h1 h2; subst h1
+  have lem := frame_wf_by_index x j1
+  generalize zdef : Γ d@ x = z at *
+  cases lem
+  all_goals (
+    unfold Frame.get_type at j2; simp at j2
+    try (subst j2; case _ j => cases j)
+  )
+  all_goals case _ z1 z2 => subst j2; cases z1
+case allk j1 j2 ih1 ih2 =>
+  intro h; cases h; case _ h1 h2 =>
+  rw [Option.bind_eq_some]; apply Exists.intro ()
+  apply And.intro (ih1 h1)
+  rw [Option.bind_eq_some]; apply Exists.intro ()
+  apply And.intro (ih2 h2) rfl
+case appk j1 j2 ih1 ih2 =>
+  intro h1 h2; subst h1
+  have lem := super_kind_shape_lemma j1; simp at lem
+  apply lem.2
+  apply Term.Subexpr.ctor2_2
+  apply Term.Subexpr.refl
+case ite j1 j2 ih1 ih2 ih3 ih4 ih5 ih6 =>
+  intro h1 h2; subst h1
+  cases j1
+case guard j ih1 ih2 ih3 ih4 ih5 =>
+  intro h1 h2; subst h1
+  cases j
+case app j1 j2 j3 ih1 ih2 =>
+  intro h1 h2; subst h1
+  have lem := super_kind_equal_beta j3
+  cases lem
+  case _ lem =>
+    subst lem
+    have lem := super_kind_shape_lemma j1; simp at lem
+    apply lem.2
+    apply @Term.Subexpr.bind2_2 _ □ _ _ _; simp
+    apply Term.Subexpr.refl
+  case _ lem =>
+    cases lem; case _ e1 e2 =>
+    subst e1; subst e2
+    cases h2; case _ j _ => cases j
+case appt j1 j2 j3 ih1 ih2 =>
+  intro h1 h2; subst h1
+  have lem := super_kind_equal_beta j3
+  cases lem
+  case _ lem =>
+    subst lem
+    have lem := super_kind_shape_lemma j1; simp at lem
+    apply lem.2
+    apply @Term.Subexpr.bind2_2 _ □ _ _ _; simp
+    apply Term.Subexpr.refl
+  case _ lem =>
+    cases lem; case _ e1 e2 =>
+    subst e1; subst e2
+    cases h2; case _ j _ => cases j
+case cast j1 j2 ih1 ih2 =>
+  intro h j; subst h
+  have lem := super_kind_shape_lemma j2; simp at lem
+  apply lem.2
+  apply Term.Subexpr.eq3
+  apply Term.Subexpr.refl
+case empty j _ _ =>
+  intro h _; subst h
+  cases j
+case choice j1 j2 j3 j4 ih1 ih2 ih3 ih4 =>
+  intro h1 h2; subst h1
+  cases j2
